examples/ghc/theories/VarEnv.v
@@ -1,3 +1,6 @@
+From mathcomp.ssreflect
+Require Import ssreflect ssrnat prime ssrbool eqtype.
+
 Require Import Coq.Lists.List.
 
 Require Import GHC.Base.
@@ -10,6 +13,7 @@ Require Import Proofs.Core.
 Require Import Proofs.Var.
 Require Import Proofs.Unique.
 Require Import Proofs.VarSet.
+Require Import Proofs.VarSetFSet.
 
 Set Bullet Behavior "Strict Subproofs".
 
@@ -154,13 +158,13 @@ Ltac rewrite_minusDom_true :=
       context [ lookupVarSet 
                   (minusDom ?s ?init_env) ?var ] ] =>  
     unfold minusDom;
-    repeat rewrite lookupVarSet_filterVarSet_false with 
+    repeat rewrite -> lookupVarSet_filterVarSet_false with 
         (f := (fun v0 : Var => negb (elemVarEnv v0 init_env ))); try rewrite H; auto 
   | [ H : elemVarEnv ?var ?init_env = true, 
           H2: context [ lookupVarSet 
                           (minusDom ?s ?init_env) ?var ] |- _ ] =>  
     unfold minusDom in H2;
-    rewrite lookupVarSet_filterVarSet_false with
+    rewrite -> lookupVarSet_filterVarSet_false with
         (f := (fun v0 : Var => negb (elemVarEnv v0 init_env ))) in H2; 
     try rewrite H; auto 
                                                                     
@@ -172,14 +176,14 @@ Ltac rewrite_minusDom_false :=
       context [ lookupVarSet 
                   (minusDom ?s ?init_env) ?var ] ] =>  
     unfold minusDom;
-    repeat rewrite lookupVarSet_filterVarSet_true
+    repeat rewrite -> lookupVarSet_filterVarSet_true
     with (f := (fun v0 : Var => negb (elemVarEnv v0 init_env ))); 
     try rewrite H; auto 
   | [ H : elemVarEnv ?var ?init_env = false, 
           H2: context [ lookupVarSet 
                           (minusDom ?s ?init_env) ?var ] |- _ ] =>  
     unfold minusDom in H2;
-    rewrite lookupVarSet_filterVarSet_true with 
+    rewrite -> lookupVarSet_filterVarSet_true with 
         (f := (fun v0 : Var => negb (elemVarEnv v0 init_env ))) in H2 ; 
     try rewrite H; auto  
   end.
@@ -207,7 +211,7 @@ Proof.
   intros.
   rewrite <- lookupVarEnv_elemVarEnv_false in H.
   unfold minusDom.
-  rewrite lookupVarSet_filterVarSet_true
+  rewrite -> lookupVarSet_filterVarSet_true
     with (f := (fun v0 : Var => negb (elemVarEnv v0 env))).
   auto.
   rewrite H. simpl. auto.
@@ -261,13 +265,15 @@ Proof.
   destruct (elemVarEnv v' env) eqn:Eenv; auto.
   + (* v' is in dom of env. so cannot be looked up. *)
     unfold minusDom.
-    rewrite 2 lookupVarSet_filterVarSet_false; auto.  
+    rewrite -> lookupVarSet_filterVarSet_false; auto.  
+    rewrite -> lookupVarSet_filterVarSet_false; auto.  
     rewrite Eenv. simpl. auto.
     rewrite elemVarEnv_extendVarEnv_neq.
     rewrite Eenv. simpl. auto.
     auto.
   + unfold minusDom.
-    rewrite 2 lookupVarSet_filterVarSet_true; auto.  
+    rewrite -> lookupVarSet_filterVarSet_true; auto.  
+    rewrite -> lookupVarSet_filterVarSet_true; auto.  
     rewrite lookupVarSet_extendVarSet_neq; auto.
     auto.
     rewrite Eenv. simpl. auto.
@@ -296,7 +302,7 @@ Proof.
   intros.
   intro var.
   destruct (var == v) eqn:EQ.
-  rewrite lookupVarSet_eq with (v2 := v); auto.
+  rewrite -> lookupVarSet_eq with (v2 := v); auto.
   unfold minusDom.
   rewrite lookupVarSet_filterVarSet_false. 
   auto.
@@ -366,3 +372,43 @@ Proof.
   f_equal.
   omega.
 Qed.
+
+
+
+
+
+
+Lemma elemVarSet_minusDom_1
+     : forall (a : Type) (env : VarEnv a) (vs : VarSet) (v : Var),
+       lookupVarEnv env v = None ->
+       elemVarSet v (minusDom vs env) = elemVarSet v vs.
+Admitted.
+
+Lemma elemVarSet_minusDom_inDom
+     : forall (a : Type) (vs : VarSet) (env : VarEnv a) (v' : Var),
+       elemVarEnv v' env -> ~~ (elemVarSet v' (minusDom vs env)).
+Admitted.
+
+Lemma Subset_minusDom {a} : forall vs1 vs2 (e: VarEnv a), 
+    vs1 [<=] vs2 ->
+    minusDom vs1 e [<=] minusDom vs2 e.
+Proof.
+  intros. 
+  unfold Subset,List.In in *.
+  intros var.
+Admitted.
+
+
+Lemma elemVarSet_minusDom_elemVarEnv : forall a vs (env:VarEnv a) v,
+    elemVarEnv v env ->
+    elemVarSet v (minusDom vs env) = false.
+Proof.
+  intros.
+Admitted.
+
+Lemma elemVarSet_minusDom_elemVarEnv_false : forall a vs (env:VarEnv a) v,
+    elemVarEnv v env = false ->
+    elemVarSet v (minusDom vs env) = elemVarSet v vs.
+Proof.
+  intros.
+Admitted.
